Updates

vale/code/lib/transformers/Vale.Transformers.LiveAnalysis.fst
@@ -1,5 +1,7 @@
 module Vale.Transformers.LiveAnalysis
 
+open FStar.Calc
+
 open Vale.X64.Bytes_Code_s
 open Vale.X64.Instruction_s
 open Vale.X64.Instructions_s
@@ -12,6 +14,8 @@ open Vale.Transformers.Locations
 open Vale.Transformers.BoundedInstructionEffects
 
 module L = FStar.List.Tot
+
+let implies x y = x ==> y
 
 (* TODO: Is there a built-in for this? *)
 irreducible
@@ -80,3 +84,222 @@ and live_of_codes (c:codes) (post:locations) : locations =
   | [] -> post
   | x :: xs ->
     live_of_code x (live_of_codes xs post)
+
+(* REVIEW: There are some similarities of the following portion with
+           the InstructionReorder module. Break out the common parts into a
+           separate module? *)
+let unchanged_at' (locs:locations) (s1 s2:machine_state) =
+  (s1.ms_ok = s2.ms_ok) /\
+  (s1.ms_ok ==>
+   unchanged_at locs s1 s2)
+
+unfold
+let erroring_option_state (s:option machine_state) =
+  match s with
+  | None -> true
+  | Some s -> not (s.ms_ok)
+
+let unchanged_at'' (locs:locations) (s1 s2:option machine_state) =
+  (erroring_option_state s1 == erroring_option_state s2) /\
+  (not (erroring_option_state s1) ==>
+   unchanged_at' locs (Some?.v s1) (Some?.v s2))
+
+let rec lemma_not_ok_propagate_code (c:code) (fuel:nat) (s:machine_state) :
+  Lemma
+    (requires (not s.ms_ok))
+    (ensures (erroring_option_state (machine_eval_code c fuel s)))
+    (decreases %[fuel; c; 1]) =
+  match c with
+  | Ins _ -> ()
+  | Block l ->
+    lemma_not_ok_propagate_codes l fuel s
+  | IfElse ifCond ifTrue ifFalse ->
+    let (st, b) = machine_eval_ocmp s ifCond in
+    let s' = {st with ms_trace = (BranchPredicate b)::s.ms_trace} in
+    if b then lemma_not_ok_propagate_code ifTrue fuel s' else lemma_not_ok_propagate_code ifFalse fuel s'
+  | While _ _ ->
+    lemma_not_ok_propagate_while c fuel s
+
+and lemma_not_ok_propagate_codes (l:codes) (fuel:nat) (s:machine_state) :
+  Lemma
+    (requires (not s.ms_ok))
+    (ensures (erroring_option_state (machine_eval_codes l fuel s)))
+    (decreases %[fuel; l]) =
+  match l with
+  | [] -> ()
+  | x :: xs ->
+    lemma_not_ok_propagate_code x fuel s;
+    match machine_eval_code x fuel s with
+    | None -> ()
+    | Some s -> lemma_not_ok_propagate_codes xs fuel s
+
+and lemma_not_ok_propagate_while (c:code{While? c}) (fuel:nat) (s:machine_state) :
+  Lemma
+    (requires (not s.ms_ok))
+    (ensures (erroring_option_state (machine_eval_code c fuel s)))
+    (decreases %[fuel; c; 0]) =
+  if fuel = 0 then () else (
+    let While cond body = c in
+    let (s, b) = machine_eval_ocmp s cond in
+    if not b then () else (
+      let s = { s with ms_trace = (BranchPredicate true) :: s.ms_trace } in
+      lemma_not_ok_propagate_code body (fuel - 1) s
+    )
+  )
+
+let rec lemma_unchanged_at'_intro (locs:locations) (s1 s2:machine_state) :
+  Lemma
+    (requires (
+        (s1.ms_ok = s2.ms_ok) /\
+        (forall x. {:pattern (L.mem x locs)} s1.ms_ok /\ L.mem x locs ==> eval_location x s1 == eval_location x s2)))
+    (ensures (unchanged_at' locs s1 s2)) =
+  match locs with
+  | [] -> ()
+  | x :: xs ->
+    assert (L.mem x locs); (* OBSERVE *)
+    assert (forall x. L.mem x xs ==> L.mem x locs); (* OBSERVE *)
+    lemma_unchanged_at'_intro xs s1 s2
+
+let rec lemma_unchanged_at'_elim (locs:locations) (s1 s2:machine_state) :
+  Lemma
+    (requires (unchanged_at' locs s1 s2))
+    (ensures (forall x. {:pattern (L.mem x locs)} s1.ms_ok /\ L.mem x locs ==> eval_location x s1 == eval_location x s2)) =
+  match locs with
+  | [] -> ()
+  | x :: xs ->
+    lemma_unchanged_at'_elim xs s1 s2
+
+let lemma_unchanged_at'_smaller (locs locs_smaller:locations) (s1 s2:machine_state) :
+  Lemma
+    (requires (
+        (unchanged_at' locs s1 s2) /\
+        (forall x. L.mem x locs_smaller ==> L.mem x locs)))
+    (ensures (unchanged_at' locs_smaller s1 s2)) =
+  lemma_unchanged_at'_elim locs s1 s2;
+  lemma_unchanged_at'_intro locs_smaller s1 s2
+
+let rec lemma_live_of_code (c:code) (post:locations) (fuel:nat) (s1 s2:machine_state) :
+  Lemma
+    (requires (unchanged_at' (live_of_code c post) s1 s2))
+    (ensures (unchanged_at'' post
+                (machine_eval_code c fuel s1)
+                (machine_eval_code c fuel s2)))
+    (decreases %[c; fuel; 1]) =
+  let pre = live_of_code c post in
+  if s1.ms_ok then (
+    match c with
+    | Ins i ->
+      admit () (* TODO: Prove *)
+    | Block l ->
+      lemma_live_of_codes l post fuel s1 s2
+    | IfElse c t f ->
+      lemma_unchanged_at'_smaller pre (locations_of_ocmp c) s1 s2;
+      lemma_locations_of_ocmp c s1 s2;
+      let st1, b1 = machine_eval_ocmp s1 c in
+      let st2, b2 = machine_eval_ocmp s2 c in
+      assert (unchanged_at' pre st1 st2);
+      assert (b1 = b2);
+      let s1' = { st1 with ms_trace = (BranchPredicate b1) :: st1.ms_trace } in
+      let s2' = { st2 with ms_trace = (BranchPredicate b2) :: st2.ms_trace } in
+      lemma_locations_same_with_filter st1 s1'.ms_flags s1'.ms_ok s1'.ms_trace;
+      lemma_locations_same_with_filter st2 s2'.ms_flags s2'.ms_ok s2'.ms_trace;
+      assert (FunctionalExtensionality.feq
+                (filter_state st1 s1'.ms_flags s1'.ms_ok s1'.ms_trace).ms_flags
+                s1'.ms_flags); (* OBSERVE *)
+      assert (FunctionalExtensionality.feq
+                (filter_state st2 s2'.ms_flags s2'.ms_ok s2'.ms_trace).ms_flags
+                s2'.ms_flags); (* OBSERVE *)
+      lemma_unchanged_at'_elim pre st1 st2;
+      lemma_unchanged_at'_intro pre s1' s2';
+      assert (unchanged_at' pre s1' s2');
+      if b1 then (
+        lemma_unchanged_at'_smaller pre (live_of_code t post) s1' s2';
+        lemma_live_of_code t post fuel s1' s2'
+      ) else (
+        lemma_unchanged_at'_smaller pre (live_of_code f post) s1' s2';
+        lemma_live_of_code f post fuel s1' s2'
+      )
+    | While _ _ ->
+      lemma_live_of_while c post fuel s1 s2
+  ) else (
+    lemma_not_ok_propagate_code c fuel s1;
+    lemma_not_ok_propagate_code c fuel s2
+  )
+
+and lemma_live_of_codes (c:codes) (post:locations) (fuel:nat) (s1 s2:machine_state) :
+  Lemma
+    (requires (unchanged_at' (live_of_codes c post) s1 s2))
+    (ensures (unchanged_at'' post
+                (machine_eval_codes c fuel s1)
+                (machine_eval_codes c fuel s2)))
+    (decreases %[c; fuel]) =
+  match c with
+  | [] -> ()
+  | x :: xs ->
+    lemma_live_of_code x (live_of_codes xs post) fuel s1 s2;
+    match machine_eval_code x fuel s1, machine_eval_code x fuel s2 with
+    | None, None -> ()
+    | Some s1', None -> lemma_not_ok_propagate_codes xs fuel s1'
+    | None, Some s2' -> lemma_not_ok_propagate_codes xs fuel s2'
+    | Some s1', Some s2' ->
+      lemma_live_of_codes xs post fuel s1' s2'
+
+and lemma_live_of_while (c:code{While? c}) (post:locations) (fuel:nat) (s1 s2:machine_state) :
+  Lemma
+    (requires (unchanged_at' (live_of_code c post) s1 s2))
+    (ensures (unchanged_at'' (live_of_code c post) (* Stronger than just for [post] *)
+                (machine_eval_code c fuel s1)
+                (machine_eval_code c fuel s2) /\
+              unchanged_at'' post
+                (machine_eval_code c fuel s1)
+                (machine_eval_code c fuel s2)))
+    (decreases %[c; fuel; 0]) =
+  let pre = live_of_code c post in
+  if s1.ms_ok then (
+    if fuel = 0 then () else (
+      let While cond body = c in
+      lemma_unchanged_at'_smaller pre (locations_of_ocmp cond) s1 s2;
+      lemma_locations_of_ocmp cond s1 s2;
+      let (s01, b1) = machine_eval_ocmp s1 cond in
+      let (s02, b2) = machine_eval_ocmp s2 cond in
+      assert (b1 = b2);
+      if not b1 then (
+        let s01' = {s01 with ms_trace = (BranchPredicate false)::s01.ms_trace} in
+        let s02' = {s02 with ms_trace = (BranchPredicate false)::s02.ms_trace} in
+        assert (unchanged_at' pre s01 s02);
+        assert ((FunctionalExtensionality.feq
+                   (filter_state s01 s01'.ms_flags s01'.ms_ok s01'.ms_trace).ms_flags
+                   s01'.ms_flags) /\
+                (FunctionalExtensionality.feq
+                   (filter_state s02 s02'.ms_flags s02'.ms_ok s02'.ms_trace).ms_flags
+                   s02'.ms_flags)); (* OBSERVE *)
+        lemma_locations_same_with_filter s01 s01'.ms_flags s01'.ms_ok s01'.ms_trace;
+        lemma_locations_same_with_filter s02 s02'.ms_flags s02'.ms_ok s02'.ms_trace;
+        lemma_unchanged_at'_elim pre s01 s02;
+        lemma_unchanged_at'_intro pre s01' s02';
+        lemma_unchanged_at'_smaller pre post s01' s02'
+      ) else (
+        let s01' = {s01 with ms_trace = (BranchPredicate true)::s01.ms_trace} in
+        let s02' = {s02 with ms_trace = (BranchPredicate true)::s02.ms_trace} in
+        assert (unchanged_at' pre s01 s02);
+        assert ((FunctionalExtensionality.feq
+                   (filter_state s01 s01'.ms_flags s01'.ms_ok s01'.ms_trace).ms_flags
+                   s01'.ms_flags) /\
+                (FunctionalExtensionality.feq
+                   (filter_state s02 s02'.ms_flags s02'.ms_ok s02'.ms_trace).ms_flags
+                   s02'.ms_flags));
+        lemma_locations_same_with_filter s01 s01'.ms_flags s01'.ms_ok s01'.ms_trace;
+        lemma_locations_same_with_filter s02 s02'.ms_flags s02'.ms_ok s02'.ms_trace;
+        lemma_unchanged_at'_elim pre s01 s02;
+        lemma_unchanged_at'_intro pre s01' s02';
+        assert (unchanged_at' pre s01' s02'); (* OBSERVE *)
+        admit ();
+        (* The proof below won't ever work since we don't take a fixpoint :/ *)
+        lemma_live_of_code body pre (fuel-1) s01' s02';
+        admit ()
+      )
+    )
+  ) else (
+    lemma_not_ok_propagate_code c fuel s1;
+    lemma_not_ok_propagate_code c fuel s2
+  )
